ContextTyping/theories/Soundness.v
@@ -18,9 +18,6 @@ From ContextBasicDenotation Require Import StoreTyping TermExtension TermTLet Qu
   BasicTypingFormula RelevantEnv.
 From Denotation Require Import Context
   TypeEquivCore
-  TypeEquivBody
-  TypeEquivArrow
-  TypeEquivWand
   TypeEquiv
   ConstDenote.
 From ContextTyping Require Import PrimOpContext Typing SoundnessLam SoundnessApp SoundnessAppD
