ContextTyping/theories/SoundnessFix.v
@@ -11,9 +11,6 @@ From ContextBasicDenotation Require Import StoreTyping TermExtension TermTLet Qu
   BasicTypingFormula RelevantEnv.
 From Denotation Require Import Context
   TypeEquivCore
-  TypeEquivBody
-  TypeEquivArrow
-  TypeEquivWand
   TypeEquiv
   ConstDenote.
 From ContextTyping Require Import Typing SoundnessLam SoundnessFixBase
