ContextTyping/theories/SoundnessFixBase.v
@@ -13,10 +13,7 @@ From ContextBasicDenotation Require Import StoreTyping TermExtension TermTLet Qu
   BasicTypingFormula RelevantEnv.
 From Denotation Require Import Context
   TypeEquivCore
-  TypeEquivBody
   TypeEquivTerm
-  TypeEquivArrow
-  TypeEquivWand
   TypeEquiv
   ConstDenote.
 From ContextTyping Require Import Typing SoundnessLam.
