ContextTyping/theories/SoundnessLam.v
@@ -13,9 +13,6 @@ From ContextBasicDenotation Require Import StoreTyping TermExtension TermTLet Qu
 From Denotation Require Import Context
   TypeEquivCore
   TypeEquivTerm
-  TypeEquivBody
-  TypeEquivArrow
-  TypeEquivWand
   TypeEquiv
   ConstDenote.
 From ContextTyping Require Import Typing.
